proofs/fstar/extraction-edited/Libcrux.Kem.Kyber.Matrix.fst
@@ -3,110 +3,128 @@ module Libcrux.Kem.Kyber.Matrix
 open Core
 open FStar.Mul
 
-let op_Array_Access (x:Libcrux.Kem.Kyber.Arithmetic.t_PolynomialRingElement) (i:usize{v i < 256}): i32  =
+open Libcrux.Kem.Kyber.Arithmetic
+
+let op_Array_Access (x:Libcrux.Kem.Kyber.Arithmetic.wfPolynomialRingElement) (i:usize{v i < 256}): i32  =
     x.f_coefficients.[i]
     
 
+#push-options "--ifuel 0 --z3rlimit 700"
 let compute_As_plus_e v_K matrix_A s_as_ntt error_as_ntt =
-  let result:t_Array Libcrux.Kem.Kyber.Arithmetic.wfPolynomialRingElement v_K =
+  let result:t_Array wfPolynomialRingElement v_K =
     Rust_primitives.Hax.repeat (Libcrux.Kem.Kyber.Arithmetic.cast_poly_b #1 #3328 Libcrux.Kem.Kyber.Arithmetic.impl__PolynomialRingElement__ZERO) v_K
   in
-  admit();
-  let acc_t = t_Array Libcrux.Kem.Kyber.Arithmetic.wfPolynomialRingElement v_K in
   [@ inline_let]
-  let inv = fun (acc:acc_t) (i:usize) -> True in
-  let result:t_Array Libcrux.Kem.Kyber.Arithmetic.wfPolynomialRingElement v_K =
-    Rust_primitives.Iterators.foldi_slice #(t_Array Libcrux.Kem.Kyber.Arithmetic.wfPolynomialRingElement v_K) #acc_t #inv
+  let inv0 = fun (acc:t_Array wfPolynomialRingElement v_K) (i:usize) -> 
+   (v i <= v v_K) /\
+   (forall (j k:usize). (v j >= v i /\ v j < v v_K /\ v k < 256) ==> v (((acc.[j] <: Libcrux.Kem.Kyber.Arithmetic.wfPolynomialRingElement).f_coefficients.[k]) <: i32) == 0)
+  in
+  let result:t_Array wfPolynomialRingElement v_K =
+    Rust_primitives.Iterators.foldi_slice #(t_Array Libcrux.Kem.Kyber.Arithmetic.wfPolynomialRingElement v_K) #(t_Array wfPolynomialRingElement v_K) #inv0
       matrix_A
       result
       (fun result temp_1_ ->
-          let result:t_Array Libcrux.Kem.Kyber.Arithmetic.wfPolynomialRingElement v_K = result in
+          let orig_result = result in
+          let orig_result_cast = (cast_vector_b #v_K #3328 #(v v_K * 3328) orig_result) in
           let i, row:(usize & t_Array Libcrux.Kem.Kyber.Arithmetic.wfPolynomialRingElement v_K) =
             temp_1_
           in
           [@ inline_let]
-          let inv = fun (acc:acc_t) (i:usize) -> True in
-          let result:t_Array Libcrux.Kem.Kyber.Arithmetic.wfPolynomialRingElement v_K =
-            Rust_primitives.Iterators.foldi_slice #Libcrux.Kem.Kyber.Arithmetic.wfPolynomialRingElement #acc_t #inv
+          let inv1 = fun (acc:t_Array (Libcrux.Kem.Kyber.Arithmetic.t_PolynomialRingElement_b (v v_K * 3328)) v_K) (inner:usize) ->
+             (v inner <= v v_K) /\
+             (forall (j:usize). (v j < v i /\ v j < v v_K) ==> acc.[j] == orig_result_cast.[j]) /\
+             (forall (j:usize). (v j > v i /\ v j < v v_K) ==> acc.[j] == orig_result_cast.[j]) /\
+             (poly_range (acc.[i] <: Libcrux.Kem.Kyber.Arithmetic.t_PolynomialRingElement_b (v v_K * 3328)) (v inner * 3328))
+          in
+          assert (forall (k:usize). (v k < 256) ==> v (result.[i] <: wfPolynomialRingElement).f_coefficients.[k] == 0);
+          assert(inv1 orig_result_cast (sz 0));
+          let result:t_Array (Libcrux.Kem.Kyber.Arithmetic.t_PolynomialRingElement_b (v v_K * 3328)) v_K =
+            Rust_primitives.Iterators.foldi_slice #Libcrux.Kem.Kyber.Arithmetic.wfPolynomialRingElement #(t_Array (Libcrux.Kem.Kyber.Arithmetic.t_PolynomialRingElement_b (v v_K * 3328)) v_K) #inv1
               row
-              result
+              orig_result_cast
               (fun result temp_1_ ->
-                  let result:t_Array Libcrux.Kem.Kyber.Arithmetic.wfPolynomialRingElement v_K =
-                    result
-                  in
                   let j, matrix_element:(usize &
                     Libcrux.Kem.Kyber.Arithmetic.wfPolynomialRingElement) =
                     temp_1_
                   in
+                  let resulti = down_cast_poly_b #(v v_K * 3328) #(v j * 3328) result.[i] in
                   let product:Libcrux.Kem.Kyber.Arithmetic.wfPolynomialRingElement =
                     Libcrux.Kem.Kyber.Ntt.ntt_multiply matrix_element
                       (s_as_ntt.[ j ] <: Libcrux.Kem.Kyber.Arithmetic.wfPolynomialRingElement)
                   in
-                  admit(); // needs bounds for add_to_ring_element
-                  let result:t_Array Libcrux.Kem.Kyber.Arithmetic.wfPolynomialRingElement v_K =
+                  let product_sum:Libcrux.Kem.Kyber.Arithmetic.t_PolynomialRingElement_b ((v j + 1) * 3328)  =
+                      (Libcrux.Kem.Kyber.Arithmetic.add_to_ring_element #(v j * 3328) #3328 v_K
+                          resulti
+                          product) in
+                  let product_sum:(Libcrux.Kem.Kyber.Arithmetic.t_PolynomialRingElement_b (v v_K * 3328)) = cast_poly_b #((v j+1)* 3328) #(v v_K * 3328) product_sum in 
+                  let result:t_Array (Libcrux.Kem.Kyber.Arithmetic.t_PolynomialRingElement_b (v v_K * 3328)) v_K =
                     Rust_primitives.Hax.Monomorphized_update_at.update_at_usize result
                       i
-                      (Libcrux.Kem.Kyber.Arithmetic.add_to_ring_element v_K
-                          (result.[ i ] <: Libcrux.Kem.Kyber.Arithmetic.wfPolynomialRingElement)
-                          product
-                        <:
-                        Libcrux.Kem.Kyber.Arithmetic.wfPolynomialRingElement)
+                      product_sum
                   in
                   result)
           in
-          let acc_t = t_Array Libcrux.Kem.Kyber.Arithmetic.wfPolynomialRingElement v_K in
+          let result1 = result in
           [@ inline_let]
-          let inv = fun (acc:acc_t) (i:usize) -> True in
-            Rust_primitives.Iterators.foldi_range #_ #acc_t #inv {
+          let inv2 = fun (acc:t_Array (Libcrux.Kem.Kyber.Arithmetic.t_PolynomialRingElement_b (v v_K * 3328)) v_K) (inner:usize) -> 
+             (v inner <= 256) /\
+             (forall (j:usize). (v j < v i /\ v j < v v_K) ==> acc.[j] == orig_result_cast.[j]) /\
+             (forall (j:usize). (v j > v i /\ v j < v v_K) ==> acc.[j] == orig_result_cast.[j]) /\
+             (forall (j:usize). (v j < v inner) ==> (i32_range (acc.[i] <: Libcrux.Kem.Kyber.Arithmetic.t_PolynomialRingElement_b (v v_K * 3328)).f_coefficients.[j] 3328))
+             // And all indexes above v inner are unchanged from result1
+          in
+          assert (inv2 result1 (sz 0));
+          let result:t_Array (Libcrux.Kem.Kyber.Arithmetic.t_PolynomialRingElement_b (v v_K * 3328)) v_K =
+            Rust_primitives.Iterators.foldi_range #_ #(t_Array (Libcrux.Kem.Kyber.Arithmetic.t_PolynomialRingElement_b (v v_K * 3328)) v_K) #inv2 {
               Core.Ops.Range.f_start = sz 0;
               Core.Ops.Range.f_end = Libcrux.Kem.Kyber.Constants.v_COEFFICIENTS_IN_RING_ELEMENT
             }
             result
-            (fun result j ->
-                let result:t_Array Libcrux.Kem.Kyber.Arithmetic.wfPolynomialRingElement v_K =
-                  result
-                in
+            (fun result j -> 
+                let result: t_Array (Libcrux.Kem.Kyber.Arithmetic.t_PolynomialRingElement_b (v v_K * 3328)) v_K = result in
                 let j:usize = j in
-                assume (range (v (result.[i]).(j) * 1353) i32_inttype);
-                let coefficient_normal_form =
-                  Libcrux.Kem.Kyber.Arithmetic.to_standard_domain #3328 ((result.[ i ]
-                        <:
-                        Libcrux.Kem.Kyber.Arithmetic.wfPolynomialRingElement)
+                let resulti:(Libcrux.Kem.Kyber.Arithmetic.t_PolynomialRingElement_b (v v_K * 3328)) = result.[ i ]  <:  (Libcrux.Kem.Kyber.Arithmetic.t_PolynomialRingElement_b (v v_K * 3328)) in
+                let coefficient_normal_form: i32_b ((nat_div_ceil (v v_K * 3328 * 1353) (pow2 16)) + 1665) =
+                  Libcrux.Kem.Kyber.Arithmetic.to_standard_domain #(v v_K * 3328) (resulti
                         .Libcrux.Kem.Kyber.Arithmetic.f_coefficients.[ j ])
                 in
-                let x1: Libcrux.Kem.Kyber.Arithmetic.wfPolynomialRingElement = error_as_ntt.[i] in
-                let x2 : i32 = x1.f_coefficients.[j] in
-                assume (range (v coefficient_normal_form + v x2) i32_inttype);
+                assert ((nat_div_ceil (v v_K * 3328 * 1353) (pow2 16)) + 1665 <= 1940);
+                let coefficient_normal_form: i32_b 1940 = cast_i32_b #((nat_div_ceil (v v_K * 3328 * 1353) (pow2 16)) + 1665)  #1940 coefficient_normal_form in
+                let x1: i32_b 3328 = (error_as_ntt.[ i ]
+                                  <:
+                                  Libcrux.Kem.Kyber.Arithmetic.wfPolynomialRingElement)
+                                  .Libcrux.Kem.Kyber.Arithmetic.f_coefficients.[ j ] in
+                let x2: i32_b 5268 = add_i32_b coefficient_normal_form x1 in
+                assert (5268 <= v v_BARRETT_R /\ v v_BARRETT_R < pow2 31);
+                let x3: i32_b (v v_BARRETT_R) = cast_i32_b #5268 #(v v_BARRETT_R) x2 in
+                let resultij: i32_b 3328 =  Libcrux.Kem.Kyber.Arithmetic.barrett_reduce x3 in
+                let resultij: i32_b (v v_K * 3328) =  cast_i32_b #3328 #(v v_K * 3328) resultij in
+                let resulti_coeffs =
+                  Rust_primitives.Hax.Monomorphized_update_at.update_at_usize
+                   (resulti.Libcrux.Kem.Kyber.Arithmetic.f_coefficients)
+                    j resultij in
+                let result = 
                 Rust_primitives.Hax.Monomorphized_update_at.update_at_usize result
                   i
                   ({
-                      (result.[ i ] <: Libcrux.Kem.Kyber.Arithmetic.wfPolynomialRingElement) with
+                      resulti with
                       Libcrux.Kem.Kyber.Arithmetic.f_coefficients
-                      =
-                      Rust_primitives.Hax.Monomorphized_update_at.update_at_usize (result.[ i ]
-                          <:
-                          Libcrux.Kem.Kyber.Arithmetic.wfPolynomialRingElement)
-                          .Libcrux.Kem.Kyber.Arithmetic.f_coefficients
-                        j
-                        (Libcrux.Kem.Kyber.Arithmetic.barrett_reduce (coefficient_normal_form +!
-                              ((error_as_ntt.[ i ]
-                                  <:
-                                  Libcrux.Kem.Kyber.Arithmetic.wfPolynomialRingElement)
-                                  .Libcrux.Kem.Kyber.Arithmetic.f_coefficients.[ j ]
-                                <:
-                                i32)
-                              <:
-                              i32)
-                          <:
-                          i32)
-                      <:
-                      t_Array i32 (sz 256)
+                      = resulti_coeffs
                     }
                     <:
-                    Libcrux.Kem.Kyber.Arithmetic.wfPolynomialRingElement)))
+                    Libcrux.Kem.Kyber.Arithmetic.t_PolynomialRingElement_b (v v_K*3328)) in
+                assert ((result.[i]).f_coefficients.[j] == resultij);
+                assert(inv2 result (j +! sz 1));
+                let result: x:t_Array (Libcrux.Kem.Kyber.Arithmetic.t_PolynomialRingElement_b (v v_K * 3328)) v_K{inv2 x (j +! mk_int 1)} = result in
+                result) in
+          let result: t_Array wfPolynomialRingElement v_K =
+            down_cast_vector_b #v_K #(v v_K * 3328) #3328 result in
+          admit();
+          result)
   in
   admit(); //P-F
-  result 
+  result  
+#pop-options 
 
 let compute_message #p v_K m_v secret_as_ntt u_as_ntt = 
   let result:Libcrux.Kem.Kyber.Arithmetic.wfPolynomialRingElement =
@@ -124,7 +142,6 @@ let compute_message #p v_K m_v secret_as_ntt u_as_ntt =
       (fun result i ->
           let result:Libcrux.Kem.Kyber.Arithmetic.wfPolynomialRingElement = result in
           let i:usize = i in
-          admit();
           let product:Libcrux.Kem.Kyber.Arithmetic.wfPolynomialRingElement =
             Libcrux.Kem.Kyber.Ntt.ntt_multiply (secret_as_ntt.[ i ]
                 <:
